theories/WPExamplesDetails.v
@@ -174,6 +174,17 @@ Proof using.
   hsimpl. math.
 Qed.
 
+
+
+  (* TODO [xnew details -> for proof details]
+  let Vs := list_boxer_to_dyns (>> (@nil A) 0) in 
+  applys (@xapp_record_new Vs);
+  [ skip (* TODO try reflexivity *)
+  | intros ?; solve [ false ]
+  | try reflexivity
+  | try reflexivity
+  | hsimpl; simpl List.combine; simpl; hsimpl; unfold protect ].  *)
+
 End Point.
 
 
